compiler uses loop for inputs

coq/Examples/cert.scm
@@ -2,7 +2,7 @@
   (defrole init
     (vars (ch chan) (x text) (k akey))
     (trace (send ch (enc x (invk k))))
-    (inputs ch k k (enc x (invk k)))))
+    (inputs ch k (enc x (invk k)))))
 
 (defskeleton cert
   (vars)
